.

theories/Data/Graph.v
@@ -1,12 +1,8 @@
-Require Import Stdlib.NArith.BinNat.
 Require Import PnV.Prelude.Prelude.
 Require Import PnV.Control.Category.
 Require Import PnV.Data.FiniteSet.
 Require Import PnV.Data.FiniteMap.
 Require Import PnV.Prelude.X.
-
-#[local] Abbreviation In := L.In.
-#[local] Infix "\in" := E.In : type_scope.
 
 Module GRAPH.
 
@@ -18,6 +14,9 @@ Class t : Type :=
   } as G.
 
 End GRAPH.
+
+#[local] Abbreviation In := L.In.
+#[local] Infix "\in" := E.In : type_scope.
 
 Section GraphTheory_basic1.
 
@@ -86,7 +85,7 @@ Inductive path (v : V) : V -> list V -> Prop :=
   | path_step (v0 : V) (v1 : V) (p : list V)
     (H_edge : (v0, v1) \in E)
     (H_path : v1 ---[ p ]--> v)
-    (NOT_IN : ~ In v1 p)
+    (NOT_IN : ~ In v0 (v1 :: p))
     : v0 ---[ v1 :: p ]--> v
   where " src ---[ p ]--> tgt " := (path tgt src p) : type_scope.
 
@@ -94,26 +93,24 @@ Inductive path (v : V) : V -> list V -> Prop :=
 
 Lemma path_vertices_no_dup (v0 : V) (v : V) (p : list V)
   (H_path : v0 ---[ p ]--> v)
-  : NoDup p.
+  : NoDup (v0 :: p).
 Proof.
-  induction H_path as [ | v0 v1 p H_edge H_path IH NOT_IN]; econstructor; eauto.
+  induction H_path as [ | v0 v1 p H_edge H_path IH NOT_IN]; econs; eauto. econs.
 Qed.
 
 Lemma no_dup_walk_is_path (v0 : V) (v : V) (w : list V)
-  (NO_DUP : NoDup w)
+  (NO_DUP : NoDup (v0 :: w))
   (H_walk : v0 ~~~[ w ]~~> v)
   : v0 ---[ w ]--> v.
 Proof.
-  induction H_walk as [ | v0 v1 w H_edge H_walk IH]; i.
-  - econstructor 1.
-  - econstructor 2.
-    + exact H_edge.
-    + eapply IH. now inv NO_DUP.
-    + now inv NO_DUP.
+  induction H_walk as [ | v0 v1 w H_edge H_walk IH]; i; econs.
+  - exact H_edge.
+  - eapply IH. now inv NO_DUP.
+  - now inv NO_DUP.
 Qed.
 
 Theorem path_iff_no_dup_walk (v0 : V) (v : V) (vs : list V)
-  : v0 ---[ vs ]--> v <-> (v0 ~~~[ vs ]~~> v /\ NoDup vs).
+  : v0 ---[ vs ]--> v <-> (v0 ~~~[ vs ]~~> v /\ NoDup (v0 :: vs)).
 Proof.
   split.
   - intros H_path. split.
@@ -127,11 +124,10 @@ Lemma path_app_inv (v0 : V) (v' : V) (vs1 : list V) (vs2 : list V)
   (PATH : v0 ---[ vs1 ++ vs2 ]--> v')
   : exists v, v0 ---[ vs1 ]--> v /\ v ---[ vs2 ]--> v'.
 Proof.
-  rewrite -> path_iff_no_dup_walk in PATH. destruct PATH as [WALK NO_DUP].
-  rewrite -> walk_app_iff in WALK. destruct WALK as (v&WALK1&WALK2).
-  exists v. split; rewrite -> path_iff_no_dup_walk.
-  - split; trivial. eapply NoDup_app_remove_r; eauto.
-  - split; trivial. eapply NoDup_app_remove_l; eauto.
+  revert v0 v' vs2 PATH. induction vs1 as [ | v1 vs1 IH]; simpl; i.
+  - exists v0. split; eauto.
+  - inv PATH. find* (v & PATH1 & PATH2) by IH.
+    exists v. split; eauto. econstructor 2; eauto. ii. contradiction NOT_IN. ss!.
 Qed.
 
 Section Walk_finds_Path.
@@ -142,10 +138,10 @@ Lemma mk_subpath (v0 : V) (v1 : V) (v : V) (p : list V)
   : exists p', v0 ---[ p' ]--> v1 /\ (exists p'', v1 ---[ p'' ]--> v /\ p = p' ++ p'').
 Proof.
   revert v1 ELEM. induction PATH as [ | v0 v1 p H_edge PATH IH NOT_IN]; i; inv ELEM.
-  - exists [v2]. split; eauto.
+  - exists [v2]. split; eauto. econstructor 2; eauto. ii. contradiction NOT_IN. ss!.
   - find* (p'&PATH1&p''&PATH2&EQ) by IH.
     exists (v1 :: p'). split.
-    + econstructor 2; eauto. subst p. rewrite in_app_iff in NOT_IN. tauto.
+    + econstructor 2; eauto. subst p. ii. apply NOT_IN. ss!.
     + exists p''. split; [exact PATH2 | now rewrite EQ].
 Qed.
 
@@ -159,13 +155,16 @@ Proof.
   - inv WALK. exists []. econstructor 1.
   - rewrite -> walk_app_iff in WALK. destruct WALK as (v1&WALK1&WALK2).
     inv WALK2. inv H_walk. pose proof (IH v0 v1 WALK1) as [p PATH].
-    pose proof (In_dec v' p) as [ELEM | NOT_IN].
-    + find* (p'&PATH'&_) by (mk_subpath _ _ _ _ PATH). ss!.
+    pose proof (In_dec v' (v0 :: p)) as [ELEM | NOT_IN].
+    + inv ELEM.
+      * exists []. econstructor 1.
+      * find* (p'&PATH'&_) by (mk_subpath _ _ _ _ PATH). ss!.
     + exists (p ++ [v']). rewrite -> path_iff_no_dup_walk. split.
       * rewrite -> walk_app_iff. exists v1. split.
         { now eapply path_iff_no_dup_walk. }
         { econstructor 2; eauto. }
-      * rewrite <- rev_involutive. eapply NoDup_rev.
+      * change (NoDup ((v0 :: p) ++ [v'])).
+        rewrite <- rev_involutive. eapply NoDup_rev.
         rewrite -> rev_unit. econstructor 2.
         { now rewrite <- In_rev. }
         { eapply NoDup_rev. eapply path_iff_no_dup_walk. exact PATH. }
@@ -185,7 +184,7 @@ Proof.
   rewrite path_iff_no_dup_walk in PATH.
   destruct PATH as [WALK NO_DUP]. split.
   - exact WALK.
-  - eapply L.no_dup_mk_edge_seq. exact NO_DUP.
+  - eapply L.no_dup_mk_edge_seq. now inv NO_DUP.
 Qed.
 
 Inductive Walk (v : V) : V -> Type :=
@@ -291,6 +290,215 @@ Proof.
     exists x. split; [exact x_in' | rewrite fx_iff; exact b_in].
 Qed.
 
+Section DIGRAPH_FIXEDPOINT.
+
+#[local] Notation " src '~~~[' w ']~~>*('  G  ')' tgt " := (@walk G tgt src w).
+#[local] Notation " src '---[' p ']-->*('  G  ')' tgt " := (@path G tgt src p).
+#[local] Notation " src '===[' t ']==>*('  G  ')' tgt " := (@trail G tgt src t).
+
+#[local] Infix "=~=" := (is_similar_to (Similarity := list_corresponds_to_finite_ensemble)).
+#[local] Abbreviation vertices := GRAPH.vertices.
+#[local] Abbreviation edges := GRAPH.edges.
+
+Context {G : GRAPH.t}.
+
+#[local] Abbreviation V := G.(vertices).
+#[local] Abbreviation E := G.(edges).
+
+#[local] Notation " src ~~~[ w ]~~> tgt " := (walk tgt src w) : type_scope.
+
+Context {A : Type} (seed : V -> ensemble A).
+
+Inductive gmu (x : V) : ensemble A :=
+  | gmu_seed
+    : seed x \subseteq gmu x
+  | gmu_propagated y
+    (EDGE : (x, y) \in E)
+    : gmu y \subseteq gmu x.
+
+Definition is_fixedpoint (value : V -> ensemble A) : Prop :=
+  forall x, forall a, a \in value x <-> (a \in seed x \/ (exists y, (x, y) \in E /\ a \in value y)).
+
+Theorem gmu_is_fixedpoint
+  : is_fixedpoint gmu.
+Proof.
+  intros x a. split.
+  - intros IN. induction IN as [x a SEED | x y EDGE a IN IH].
+    + now left.
+    + now right; exists y.
+  - intros [SEED | (y & EDGE & IN)].
+    + now eapply gmu_seed.
+    + eapply gmu_propagated; eauto.
+Qed.
+
+Theorem gmu_is_least_fixedpoint (value : V -> ensemble A)
+  (FIXPOINT : is_fixedpoint value)
+  : forall x, gmu x \subseteq value x.
+Proof.
+  red in FIXPOINT. intros x a IN. induction IN as [x a SEED | x y EDGE a IN IH].
+  - rewrite -> FIXPOINT with (x := x) (a := a). now left.
+  - rewrite -> FIXPOINT with (x := x) (a := a). right. exists y. split; eauto.
+Qed.
+
+Variable seed' : V -> list A.
+
+Hypothesis seed_sim : forall v, seed' v =~= seed v.
+
+Variable vertices' : list V.
+
+Definition reachable (x : V) : ensemble V :=
+  fun y => exists w, x ~~~[ w ]~~> y.
+
+Context `{V_dec : hasEqDec V} `{E_dec : forall x : V, forall y : V, B.Decision ((x, y) \in E)}.
+
+Fixpoint reachableb (fuel : nat) (x : V) (y : V) {struct fuel} : bool :=
+  match fuel with
+  | O => eqb x y
+  | S fuel' => eqb x y || L.existsb (fun z => if E_dec x z then reachableb fuel' z y else false) vertices'
+  end.
+
+Definition reachable' (x : V) : list V :=
+  x :: L.filter (reachableb (L.length vertices') x) vertices'.
+
+Lemma reachableb_elim (fuel : nat) (x : V) (y : V)
+  (REACH : reachableb fuel x y = true)
+  : exists w, L.length w <= fuel /\ x ~~~[ w ]~~> y.
+Proof.
+  revert x y REACH. induction fuel as [ | fuel IH]; i; simpl in REACH.
+  - rewrite eqb_eq in REACH. subst y.
+    exists []. split; [simpl; lia | econstructor 1].
+  - rewrite orb_true_iff in REACH. destruct REACH as [EQ | REACH].
+    + rewrite eqb_eq in EQ. subst y.
+      exists []. split; [simpl; lia | econstructor 1].
+    + rewrite -> L.existsb_exists in REACH.
+      destruct REACH as (z & z_in & REACH).
+      destruct (E_dec x z) as [EDGE | NO_EDGE]; try discriminate.
+      find (w & LENGTH & WALK) by (IH z y).
+      exists (z :: w). split; [simpl; lia | econstructor 2; eauto].
+Qed.
+
+Definition gmu' (x : V) : list A :=
+  L.flat_map seed' (reachable' x).
+
+Hypothesis vertices_edge_target : forall x, forall y, (x, y) \in E -> L.In y vertices'.
+
+Lemma walk_elem_in_vertices (x : V) (y : V) (w : list V)
+  (WALK : x ~~~[ w ]~~> y)
+  : forall z, In z w -> In z vertices'.
+Proof.
+  induction WALK as [ | v0 v1 w EDGE WALK IH]; intros z IN; inv IN; eauto.
+Qed.
+
+Lemma walk_endpoint_in_vertices (x : V) (y : V) (w : list V)
+  (WALK : x ~~~[ w ]~~> y)
+  (NE : y ≠ x)
+  : In y vertices'.
+Proof.
+  induction WALK as [ | v0 v1 w EDGE WALK IH]; eauto with *.
+  pose proof (B.decide (y = v1)) as [EQ | NE']; eauto.
+  subst y. eapply vertices_edge_target; eauto.
+Qed.
+
+Lemma reachableb_intro (fuel : nat) (x : V) (y : V) (w : list V)
+  (WALK : x ~~~[ w ]~~> y)
+  (LENGTH : L.length w <= fuel)
+  : reachableb fuel x y = true.
+Proof.
+  revert fuel LENGTH. induction WALK as [ | v0 v1 w EDGE WALK IH]; i.
+  - destruct fuel as [ | fuel]; simpl.
+    + now rewrite eqb_eq.
+    + rewrite orb_true_iff. left. now rewrite eqb_eq.
+  - destruct fuel as [ | fuel]; simpl in LENGTH; [lia | ].
+    simpl. rewrite orb_true_iff. right. rewrite L.existsb_exists.
+    exists v1. split; eauto. destruct (E_dec v0 v1) as [EDGE' | NO_EDGE]; ss!.
+Qed.
+
+Lemma reachableb_iff_reachable (x : V) (y : V)
+  : reachableb (L.length vertices') x y = true <-> y \in reachable x.
+Proof.
+  split.
+  - i.
+    find* (w & _ & WALK) by reachableb_elim.
+    now exists w.
+  - intros [w WALK].
+    assert (exists p, x ---[ p ]-->*( G ) y) as [p PATH].
+    { eapply @walk_finds_path with (G := G) (w := w); eauto.
+      now intros v vs; pose proof (L.in_dec V_dec v vs) as [YES | NO]; [left | right].
+    }
+    rewrite path_iff_no_dup_walk in PATH.
+    clear WALK. destruct PATH as [WALK NO_DUP].
+    eapply reachableb_intro; eauto.
+    eapply L.NoDup_incl_length; [now inv NO_DUP | ii].
+    eapply walk_elem_in_vertices; eauto.
+Qed.
+
+Lemma reachable_sim (x : V)
+  : reachable' x =~= reachable x.
+Proof.
+  rewrite list_corresponds_to_finite_ensemble_iff.
+  intros y. unfold reachable'. simpl. rewrite -> L.filter_In. split.
+  - intros [EQ | [_ REACH]].
+    + subst y. exists []. econstructor 1.
+    + now rewrite <- reachableb_iff_reachable.
+  - intros REACH. destruct REACH as [w WALK].
+    destruct (B.decide (y = x)) as [EQ | NE].
+    + now left.
+    + right. split.
+      * eapply walk_endpoint_in_vertices; eauto.
+      * rewrite reachableb_iff_reachable. exists w. exact WALK.
+Qed.
+
+Lemma walk_gmu (x : V) (y : V) (w : list V)
+  (WALK : x ~~~[ w ]~~> y)
+  : gmu y \subseteq gmu x.
+Proof.
+  induction WALK as [ | v0 v1 w EDGE WALK IH]; intros a IN; eauto. eapply gmu_propagated; eauto.
+Qed.
+
+Lemma reachable_seed_gmu (x : V) (y : V) (a : A)
+  (REACH : y \in reachable x)
+  (SEED : a \in seed y)
+  : a \in gmu x.
+Proof.
+  destruct REACH as [w WALK]. eapply walk_gmu; [exact WALK | now eapply gmu_seed].
+Qed.
+
+Lemma reachable_step (x : V) (y : V) (z : V)
+  (EDGE : (x, y) \in E)
+  (REACH : z \in reachable y)
+  : z \in reachable x.
+Proof.
+  destruct REACH as [w WALK]. exists (y :: w). econs 2; eauto.
+Qed.
+
+Lemma gmu_reachable_seed (x : V) (a : A)
+  (IN : a \in gmu x)
+  : exists y, y \in reachable x /\ a \in seed y.
+Proof.
+  induction IN as [x a SEED | x y EDGE a IN (z & REACH & SEED)].
+  - exists x. split; [exists []; econs 1 | auto].
+  - exists z. split; [eapply reachable_step; eauto | auto].
+Qed.
+
+Lemma gmu_iff_reachable_seed (x : V) (a : A)
+  : a \in gmu x <-> a \in (reachable x >>= seed).
+Proof.
+  split.
+  - eapply gmu_reachable_seed.
+  - intros (y & REACH & SEED). eapply reachable_seed_gmu; eauto.
+Qed.
+
+Theorem gmu_sim (x : V)
+  : gmu' x =~= gmu x.
+Proof.
+  find* H by (list_corresponds_to_finite_ensemble_flat_map (reachable' x) (reachable x)).
+  - eapply reachable_sim.
+  - rewrite list_corresponds_to_finite_ensemble_iff in H |- *.
+    i. rewrite H. symmetry. eapply gmu_iff_reachable_seed.
+Qed.
+
+End DIGRAPH_FIXEDPOINT.
+
 #[local] Hint Rewrite @L.last_cons : simplication_hints.
 #[local] Hint Constructors walk : simplication_hints.
 #[local] Hint Constructors path : simplication_hints.
@@ -386,7 +594,7 @@ Proof.
   { eapply walk_finds_path with (w := tr); auto. intros v vs.
     now pose proof (@L.in_dec X (HsOrd_implies_EqDec HsOrd_X) v vs) as [YES | NO]; [left | right].
   }
-  rewrite path_iff_no_dup_walk in PATH. destruct PATH as [WALK' NO_DUP].
+  rewrite path_iff_no_dup_walk in PATH. destruct PATH as [WALK' NO_DUP]. inv NO_DUP.
   find* ? by (propagate_walk_trace _ _ _ simple). ss!.
 Qed.
 
@@ -438,896 +646,107 @@ Proof.
   - exact (proj2 (EQUATION x a) (or_intror (@ex_intro _ _ y (conj EDGE IH)))).
 Qed.
 
-Section KLEENE.
-
-Definition table : Type :=
-  fpmap X (fset A).
-
-Definition tableGet (m : table) (x : X) : fset A :=
-  match lookup x m with
-  | Some Y => Y
-  | None => FS.empty
+Fixpoint propagate_value (fuel : nat) (x : X) : fset A :=
+  match fuel with
+  | O => seed x
+  | S fuel' => FS.union (seed x) (FS.bind (deps x) (propagate_value fuel'))
   end.
 
-Definition tableStep (m : table) (x : X) : fset A :=
-  FS.union (seed x) (FS.bind (deps x) (tableGet m)).
-
-Fixpoint tableBuild (F : X -> fset A) (xs : list X) {struct xs} : table :=
-  match xs with
-  | [] => empty
-  | x :: xs' => insert x (F x) (tableBuild F xs')
-  end.
-
-Lemma tableBuild_fold (F : X -> fset A) (xs : list X)
-  : tableBuild F xs =
-    L.fold_right (fun x => fun m => insert x (F x) m) empty xs.
+Lemma propagate_value_seed (fuel : nat) (x : X) (a : A)
+  (IN : a ∈ seed x)
+  : a ∈ propagate_value fuel x.
 Proof.
-  induction xs as [ | x xs IH]; cbn [tableBuild L.fold_right];
-    [reflexivity | now rewrite IH].
+  destruct fuel as [ | fuel]; cbn [propagate_value].
+  - exact IN.
+  - rewrite FS.in_union_iff. left. exact IN.
 Qed.
 
-Lemma lookup_tableBuild_in (F : X -> fset A) (xs : list X) (x : X)
-  (IN : L.In x xs)
-  : lookup x (tableBuild F xs) = Some (F x).
-Proof.
-  induction xs as [ | x' xs IH]; simpl in IN; [contradiction | ].
-  simpl. pose proof (B.decide (x = x')) as [EQ | NE].
-  - subst x'. eapply lookup_insert_eq.
-  - rewrite lookup_insert_ne by exact NE. eapply IH.
-    destruct IN as [EQ | IN]; [contradiction NE; congruence | exact IN].
-Qed.
-
-Variable nodes : fset X.
-
-Definition propagateRow (snapshot : table) (binding : X * fset A)
-  : X * fset A :=
-  let '(x, old) := binding in
-  (x, FS.union old (FS.bind (deps x) (tableGet snapshot))).
-
-Fixpoint propagateRowsKeys (snapshot : table) (rows : list (X * fset A))
-  : map fst (map (propagateRow snapshot) rows) = map fst rows.
-Proof.
-  destruct rows as [ | [x old] rows]; cbn [map propagateRow];
-    [reflexivity | ].
-  f_equal. eapply propagateRowsKeys.
-Qed.
-
-Definition propagateSweep (m : table) : table.
-Proof.
-  refine (FiniteMap.mk (map (propagateRow m) m.(FiniteMap.data)) _).
-  rewrite propagateRowsKeys. exact m.(FiniteMap.data_isSorted).
-Defined.
-
-Local Definition propagateRowsSubset (universe : fset A) (m : table)
-  : Prop :=
-  forall (x : X) (row : fset A), lookup x m = Some row ->
-    forall a : A, a ∈ row -> a ∈ universe.
-
-Lemma propagateTableGet_subset (universe : fset A) (m : table)
-  (ROWS : propagateRowsSubset universe m) (x : X) (a : A)
-  (IN : a ∈ tableGet m x)
-  : a ∈ universe.
-Proof.
-  unfold tableGet in IN. destruct (lookup x m) as [row | ] eqn:LOOK.
-  - exact (ROWS x row LOOK a IN).
-  - contradiction IN.
-Qed.
-
-Lemma propagateSweep_lookup (m : table) (x : X) (old : fset A)
-  (LOOK : lookup x m = Some old)
-  : lookup x (propagateSweep m) =
-      Some (FS.union old (FS.bind (deps x) (tableGet m))).
-Proof.
-  rewrite lookup_spec in LOOK |- *.
-  cbn [propagateSweep FiniteMap.data].
-  rewrite L.in_map_iff. exists (x, old). split; [reflexivity | exact LOOK].
-Qed.
-
-Lemma propagateSweep_lookup_inv (m : table) (x : X) (next : fset A)
-  (LOOK : lookup x (propagateSweep m) = Some next)
-  : exists old : fset A,
-      lookup x m = Some old /\
-      next = FS.union old (FS.bind (deps x) (tableGet m)).
-Proof.
-  rewrite lookup_spec in LOOK.
-  cbn [propagateSweep FiniteMap.data] in LOOK.
-  rewrite L.in_map_iff in LOOK. destruct LOOK as [[y old] [EQ IN]].
-  cbn [propagateRow] in EQ. inversion EQ; subst y next.
-  exists old. split; [now rewrite lookup_spec | reflexivity].
-Qed.
-
-Lemma propagateSweep_rows_subset (universe : fset A) (m : table)
-  (ROWS : propagateRowsSubset universe m)
-  : propagateRowsSubset universe (propagateSweep m).
-Proof.
-  intros x next LOOK a IN.
-  destruct (propagateSweep_lookup_inv m x next LOOK)
-    as (old & LOOK_OLD & EQ). subst next.
-  rewrite FS.in_union_iff in IN. destruct IN as [IN | IN].
-  - exact (ROWS x old LOOK_OLD a IN).
-  - rewrite FS.in_bind_iff in IN. destruct IN as (y & _ & IN).
-    exact (propagateTableGet_subset universe m ROWS y a IN).
-Qed.
-
-Local Fixpoint propagateMassData (rows : list (X * fset A)) : nat :=
-  match rows with
-  | [] => O
-  | (_, row) :: rows' => length row.(FSet.data) + propagateMassData rows'
-  end.
-
-Local Definition propagateMass (m : table) : nat :=
-  propagateMassData m.(FiniteMap.data).
-
-Local Definition propagateMeasure (universe : fset A) (m : table) : nat :=
-  length m.(FiniteMap.data) * length universe.(FSet.data) -
-    propagateMass m.
-
-Lemma propagateUnion_length_le (old extra : fset A)
-  : length old.(FSet.data) <= length (FS.union old extra).(FSet.data).
-Proof.
-  eapply fset_length_le. intros a IN. rewrite FS.in_union_iff. now left.
-Qed.
-
-Lemma propagateUnion_length_lt (old extra : fset A)
-  (NE : FS.union old extra <> old)
-  : length old.(FSet.data) < length (FS.union old extra).(FSet.data).
-Proof.
-  pose proof (propagateUnion_length_le old extra) as LE.
-  assert (NE_LENGTH :
-    length old.(FSet.data) <>
-    length (FS.union old extra).(FSet.data)).
-  { intros EQ. apply NE. rewrite fset_eq_spec. intros a. split.
-    - intros IN.
-      assert (REV : forall z : A,
-        z ∈ (FS.union old extra) -> z ∈ old).
-      { eapply L.NoDup_length_incl.
-        - exact (fset_NoDup old).
-        - lia.
-        - intros z z_IN. rewrite FS.in_union_iff. now left. }
-      exact (REV a IN).
-    - intros IN. apply FS.in_union_iff. now left. }
-  lia.
-Qed.
-
-Lemma propagateSweep_mass_facts (m : table)
-  : propagateMass m <= propagateMass (propagateSweep m) /\
-    (propagateSweep m <> m ->
-      propagateMass m < propagateMass (propagateSweep m)).
-Proof.
-  unfold propagateMass. cbn [propagateSweep FiniteMap.data].
-  assert (FACTS : forall rows : list (X * fset A),
-    propagateMassData rows <=
-      propagateMassData (map (propagateRow m) rows) /\
-    (map (propagateRow m) rows <> rows ->
-      propagateMassData rows <
-        propagateMassData (map (propagateRow m) rows))).
-  { induction rows as [ | [x old] rows IH].
-    - cbn [map propagateMassData]. split;
-        [lia | intros NE; exfalso; apply NE; reflexivity].
-    - cbn [map propagateRow propagateMassData].
-      destruct IH as [TAIL_LE TAIL_LT].
-      set (extra := FS.bind (deps x) (tableGet m)).
-      pose proof (propagateUnion_length_le old extra) as HERE_LE.
-      split; [lia | ]. intros NE.
-      destruct (B.decide (FS.union old extra = old))
-        as [HERE_EQ | HERE_NE].
-      + assert (TAIL_NE : map (propagateRow m) rows <> rows).
-        { intros TAIL_EQ. apply NE. rewrite HERE_EQ, TAIL_EQ. reflexivity. }
-        pose proof (TAIL_LT TAIL_NE). lia.
-      + pose proof (propagateUnion_length_lt old extra HERE_NE). lia. }
-  destruct (FACTS m.(FiniteMap.data)) as [MASS_LE MASS_LT].
-  split; [exact MASS_LE | ]. intros CHANGED.
-  eapply MASS_LT. intros DATA_EQ. apply CHANGED.
-  apply (proj2 (FiniteMap.t_eq_iff (propagateSweep m) m)).
-  cbn [propagateSweep FiniteMap.data]. exact DATA_EQ.
-Qed.
-
-Lemma propagateMass_bound (universe : fset A) (m : table)
-  (ROWS : propagateRowsSubset universe m)
-  : propagateMass m <=
-      length m.(FiniteMap.data) * length universe.(FSet.data).
-Proof.
-  unfold propagateMass. remember m.(FiniteMap.data) as rows eqn:EQ_ROWS.
-  assert (IN_M : forall x row,
-    L.In (x, row) rows -> lookup x m = Some row).
-  { intros x row IN. rewrite lookup_spec. now rewrite <- EQ_ROWS. }
-  clear EQ_ROWS. induction rows as [ | [x row] rows IH].
-  - cbn [propagateMassData length]. lia.
-  - cbn [propagateMassData length].
-    assert (ROW_LE : length row.(FSet.data) <= length universe.(FSet.data)).
-    { eapply fset_length_le. intros a IN.
-      eapply ROWS; [eapply IN_M; now left | exact IN]. }
-    assert (TAIL : forall y row',
-      L.In (y, row') rows -> lookup y m = Some row').
-    { intros y row' IN. eapply IN_M. now right. }
-    specialize (IH TAIL). lia.
-Qed.
-
-Lemma propagateSweep_length (m : table)
-  : length (propagateSweep m).(FiniteMap.data) =
-    length m.(FiniteMap.data).
-Proof.
-  cbn [propagateSweep FiniteMap.data]. now rewrite L.length_map.
-Qed.
-
-Lemma propagateSweep_measure_lt (universe : fset A) (m : table)
-  (ROWS : propagateRowsSubset universe m)
-  (CHANGED : propagateSweep m <> m)
-  : propagateMeasure universe (propagateSweep m) <
-    propagateMeasure universe m.
-Proof.
-  pose proof (proj2 (propagateSweep_mass_facts m) CHANGED) as MASS_LT.
-  pose proof
-    (propagateMass_bound universe (propagateSweep m)
-      (propagateSweep_rows_subset universe m ROWS)) as BOUND.
-  unfold propagateMeasure. rewrite propagateSweep_length in BOUND |- *.
-  lia.
-Qed.
-
-Definition propagateStepRel (next current : table) : Prop :=
-  next = propagateSweep current /\ next <> current.
-
-Definition propagateRelAcc (universe : fset A)
-  : forall m : table,
-      propagateRowsSubset universe m ->
-      Acc Nat.lt (propagateMeasure universe m) ->
-      Acc propagateStepRel m.
-Proof.
-  refine (fix go (m : table) (ROWS : propagateRowsSubset universe m)
-    (H_Acc : Acc Nat.lt (propagateMeasure universe m)) {struct H_Acc}
-    : Acc propagateStepRel m := _).
-  constructor. intros next STEP. destruct STEP as [EQ CHANGED]. subst next.
-  exact (go (propagateSweep m) (propagateSweep_rows_subset universe m ROWS)
-    (Acc_inv H_Acc
-      (propagateSweep_measure_lt universe m ROWS CHANGED))).
-Defined.
-
-Definition propagateRun
-  : forall m : table, Acc propagateStepRel m -> table.
-Proof.
-  refine (fix go (m : table) (H_Acc : Acc propagateStepRel m)
-    {struct H_Acc} : table := _).
-  set (next := propagateSweep m).
-  destruct (B.decide (next = m)) as [SAME | CHANGED].
-  - exact m.
-  - exact (go next (Acc_inv H_Acc (conj eq_refl CHANGED))).
-Defined.
-
-Fixpoint propagateRun_fixed (m : table)
-  (H_Acc : Acc propagateStepRel m) {struct H_Acc}
-  : propagateSweep (propagateRun m H_Acc) = propagateRun m H_Acc.
-Proof.
-  destruct H_Acc as [H_Acc_inv].
-  cbn [propagateRun]. destruct (B.decide (propagateSweep m = m)).
-  - assumption.
-  - eapply propagateRun_fixed.
-Qed.
-
-Local Definition propagateUniverse : fset A :=
-  FS.bind nodes seed.
-
-Definition propagateInitial : table :=
-  tableBuild seed nodes.(FSet.data).
-
-Lemma propagateInitial_rows_subset
-  : propagateRowsSubset propagateUniverse propagateInitial.
-Proof.
-  intros x row LOOK a IN.
-  unfold propagateInitial, propagateUniverse in *.
-  rewrite tableBuild_fold in LOOK.
-  pose proof (lookup_tabulated_inv seed nodes.(FSet.data) x row LOOK)
-    as [IN_X EQ]. subst row.
-  rewrite FS.in_bind_iff. exists x. split; assumption.
-Qed.
-
-Local Definition propagateDomain (m : table) : Prop :=
-  forall x : X, x ∈ nodes -> exists row : fset A, lookup x m = Some row.
-
-Local Definition propagateKeysIn (m : table) : Prop :=
-  forall (x : X) (row : fset A), lookup x m = Some row -> x ∈ nodes.
-
-Local Definition propagateSeedIncluded (m : table) : Prop :=
-  forall (x : X) (a : A), x ∈ nodes -> a ∈ seed x ->
-    a ∈ tableGet m x.
-
-Local Definition propagateSound (m : table) : Prop :=
-  forall (x : X) (a : A), a ∈ tableGet m x ->
-    x \in propagate_closure a.
-
-Inductive propagate_closure_on (a : A) (x : X) : Prop :=
-  | propagate_closure_on_seed
-    (IN : a ∈ seed x)
-    : propagate_closure_on a x
-  | propagate_closure_on_step y
-    (EDGE : y ∈ deps x)
-    (IN_Y : y ∈ nodes)
-    (IN : propagate_closure_on a y)
-    : propagate_closure_on a x.
-
-Local Definition propagateSoundIn (m : table) : Prop :=
-  forall (x : X) (a : A), a ∈ tableGet m x ->
-    propagate_closure_on a x.
-
-Local Definition propagateInvariant (m : table) : Prop :=
-  propagateRowsSubset propagateUniverse m /\
-  propagateKeysIn m /\
-  propagateDomain m /\
-  propagateSeedIncluded m /\
-  propagateSound m /\
-  propagateSoundIn m.
-
-Lemma propagateInitial_invariant : propagateInvariant propagateInitial.
-Proof.
-  repeat split.
-  - exact propagateInitial_rows_subset.
-  - intros x row LOOK. unfold propagateInitial in LOOK.
-    rewrite tableBuild_fold in LOOK.
-    exact (proj1 (lookup_tabulated_inv seed nodes.(FSet.data) x row LOOK)).
-  - intros x IN_X. exists (seed x).
-    unfold propagateInitial. eapply lookup_tableBuild_in. exact IN_X.
-  - intros x a IN_X IN.
-    unfold tableGet, propagateInitial.
-    rewrite lookup_tableBuild_in by exact IN_X. exact IN.
-  - intros x a IN.
-    unfold tableGet, propagateInitial in IN.
-    destruct (lookup x (tableBuild seed nodes.(FSet.data)))
-      as [row | ] eqn:LOOK; [ | contradiction IN].
-    rewrite tableBuild_fold in LOOK.
-    pose proof (lookup_tabulated_inv seed nodes.(FSet.data) x row LOOK)
-      as [_ EQ]. subst row. now eapply propagate_closure_seed.
-  - intros x a IN.
-    unfold tableGet, propagateInitial in IN.
-    destruct (lookup x (tableBuild seed nodes.(FSet.data)))
-      as [row | ] eqn:LOOK; [ | contradiction IN].
-    rewrite tableBuild_fold in LOOK.
-    pose proof (lookup_tabulated_inv seed nodes.(FSet.data) x row LOOK)
-      as [_ EQ]. subst row. now eapply propagate_closure_on_seed.
-Qed.
-
-Lemma propagateSweep_invariant (m : table)
-  (INV : propagateInvariant m)
-  : propagateInvariant (propagateSweep m).
-Proof.
-  destruct INV as [ROWS [KEYS [DOMAIN [SEEDS [SOUND SOUND_IN]]]]].
-  repeat split.
-  - now apply propagateSweep_rows_subset.
-  - intros x next LOOK.
-    destruct (propagateSweep_lookup_inv m x next LOOK)
-      as (old & LOOK_OLD & _). exact (KEYS x old LOOK_OLD).
-  - intros x IN_X. destruct (DOMAIN x IN_X) as [old LOOK].
-    exists (FS.union old (FS.bind (deps x) (tableGet m))).
-    now apply propagateSweep_lookup.
-  - intros x a IN_X IN.
-    destruct (DOMAIN x IN_X) as [old LOOK].
-    unfold tableGet.
-    rewrite (propagateSweep_lookup m x old LOOK).
-    apply FS.in_union_iff. left.
-    pose proof (SEEDS x a IN_X IN) as IN_OLD.
-    unfold tableGet in IN_OLD. now rewrite LOOK in IN_OLD.
-  - intros x a IN.
-    unfold tableGet in IN.
-    destruct (lookup x (propagateSweep m)) as [next | ] eqn:LOOK;
-      [ | contradiction IN].
-    destruct (propagateSweep_lookup_inv m x next LOOK)
-      as (old & LOOK_OLD & EQ). subst next.
-    rewrite FS.in_union_iff in IN. destruct IN as [IN | IN].
-    + eapply SOUND. unfold tableGet. now rewrite LOOK_OLD.
-    + rewrite FS.in_bind_iff in IN. destruct IN as (y & EDGE & IN).
-      eapply propagate_closure_step with (y := y); [exact EDGE | ].
-      now eapply SOUND.
-  - intros x a IN.
-    unfold tableGet in IN.
-    destruct (lookup x (propagateSweep m)) as [next | ] eqn:LOOK;
-      [ | contradiction IN].
-    destruct (propagateSweep_lookup_inv m x next LOOK)
-      as (old & LOOK_OLD & EQ). subst next.
-    rewrite FS.in_union_iff in IN. destruct IN as [IN | IN].
-    + eapply SOUND_IN. unfold tableGet. now rewrite LOOK_OLD.
-    + rewrite FS.in_bind_iff in IN. destruct IN as (y & EDGE & IN).
-      eapply propagate_closure_on_step with (y := y).
-      * exact EDGE.
-      * unfold tableGet in IN. destruct (lookup y m) as [row | ] eqn:LOOK_Y;
-          [ | contradiction IN].
-        exact (KEYS y row LOOK_Y).
-      * now eapply SOUND_IN.
-Qed.
-
-Fixpoint propagateRun_invariant (m : table)
-  (H_Acc : Acc propagateStepRel m) (INV : propagateInvariant m)
-  {struct H_Acc}
-  : propagateInvariant (propagateRun m H_Acc).
-Proof.
-  destruct H_Acc as [H_Acc_inv].
-  cbn [propagateRun]. destruct (B.decide (propagateSweep m = m)).
-  - exact INV.
-  - eapply propagateRun_invariant. now apply propagateSweep_invariant.
-Qed.
-
-Definition propagateTable : table :=
-  propagateRun propagateInitial
-    (propagateRelAcc propagateUniverse propagateInitial
-      propagateInitial_rows_subset
-      (accLt (propagateMeasure propagateUniverse propagateInitial))).
-
-Lemma propagateTable_fixed
-  : propagateSweep propagateTable = propagateTable.
-Proof.
-  unfold propagateTable. apply propagateRun_fixed.
-Qed.
-
-Lemma propagateTable_invariant : propagateInvariant propagateTable.
-Proof.
-  unfold propagateTable. apply propagateRun_invariant.
-  exact propagateInitial_invariant.
-Qed.
-
-Definition propagate_kleene : X -> fset A :=
-  let m := propagateTable in
-  fun x => tableStep m x.
-
-Lemma propagateFixed_step (m : table)
-  (DOMAIN : propagateDomain m)
-  (FIXED : propagateSweep m = m)
-  (x y : X) (a : A)
-  (IN_X : x ∈ nodes)
+Lemma propagate_value_propagated (fuel : nat) (x : X) (y : X) (a : A)
   (EDGE : y ∈ deps x)
-  (IN : a ∈ tableGet m y)
-  : a ∈ tableGet m x.
+  (IN : a ∈ propagate_value fuel y)
+  : a ∈ propagate_value (S fuel) x.
 Proof.
-  destruct (DOMAIN x IN_X) as [old LOOK].
-  pose proof (propagateSweep_lookup m x old LOOK) as NEXT.
-  rewrite FIXED, LOOK in NEXT. injection NEXT as EQ.
-  unfold tableGet. rewrite LOOK, EQ.
-  apply FS.in_union_iff. right. rewrite FS.in_bind_iff.
-  exists y. split; assumption.
+  cbn [propagate_value]. rewrite FS.in_union_iff. right.
+  rewrite FS.in_bind_iff. exists y. split; assumption.
 Qed.
 
-Lemma propagateTable_complete (x : X) (a : A)
-  (IN_X : x ∈ nodes)
-  (CLOSURE : x \in propagate_closure a)
-  (deps_CLOSED : forall x : X, forall y : X, y ∈ deps x -> y ∈ nodes)
-  : a ∈ tableGet propagateTable x.
+Theorem propagate_value_elim (fuel : nat) (x : X) (a : A)
+  (IN : a ∈ propagate_value fuel x)
+  : x \in propagate_closure a.
 Proof.
-  pose proof propagateTable_invariant as
-    [_ [_ [DOMAIN [SEEDS _]]]].
-  revert IN_X. induction CLOSURE as
-    [x SEED | x y EDGE CLOSURE IH]; intros IN_X.
-  - exact (SEEDS x a IN_X SEED).
-  - eapply propagateFixed_step with (y := y).
-    + exact DOMAIN.
-    + exact propagateTable_fixed.
-    + exact IN_X.
-    + exact EDGE.
-    + eapply IH. exact (deps_CLOSED x y EDGE).
+  revert x a IN. induction fuel as [ | fuel IH]; intros x a IN; cbn [propagate_value] in IN.
+  - eapply propagate_closure_seed. exact IN.
+  - rewrite FS.in_union_iff in IN. destruct IN as [SEED_IN | BIND_IN].
+    + eapply propagate_closure_seed. exact SEED_IN.
+    + rewrite FS.in_bind_iff in BIND_IN. destruct BIND_IN as (y & EDGE & IN').
+      eapply propagate_closure_step; [exact EDGE | exact (IH y a IN')].
 Qed.
 
-Lemma propagateTable_complete_on (x : X) (a : A)
-  (IN_X : x ∈ nodes)
-  (CLOSURE : propagate_closure_on a x)
-  : a ∈ tableGet propagateTable x.
+Lemma propagate_value_monotone_step (fuel : nat) (x : X) (a : A)
+  (IN : a ∈ propagate_value fuel x)
+  : a ∈ propagate_value (S fuel) x.
 Proof.
-  pose proof propagateTable_invariant as
-    [_ [_ [DOMAIN [SEEDS _]]]].
-  revert IN_X. induction CLOSURE as
-    [x SEED | x y EDGE IN_Y CLOSURE IH]; intros IN_X.
-  - exact (SEEDS x a IN_X SEED).
-  - eapply propagateFixed_step with (y := y).
-    + exact DOMAIN.
-    + exact propagateTable_fixed.
-    + exact IN_X.
-    + exact EDGE.
-    + exact (IH IN_Y).
+  revert x a IN. induction fuel as [ | fuel IH]; intros x a IN; cbn [propagate_value] in IN |- *.
+  - rewrite FS.in_union_iff. left. exact IN.
+  - rewrite FS.in_union_iff in IN |- *. destruct IN as [SEED_IN | BIND_IN]; [now left | right].
+    rewrite FS.in_bind_iff in BIND_IN |- *. destruct BIND_IN as (y & EDGE & IN').
+    exists y. split; [exact EDGE | exact (IH y a IN')].
 Qed.
 
-Theorem propagate_kleene_iff_closure_on (x : X) (a : A)
-  : a ∈ propagate_kleene x <-> propagate_closure_on a x.
+Lemma propagate_value_monotone (fuel1 : nat) (fuel2 : nat) (x : X) (a : A)
+  (LE : fuel1 <= fuel2)
+  (IN : a ∈ propagate_value fuel1 x)
+  : a ∈ propagate_value fuel2 x.
 Proof.
-  unfold propagate_kleene, tableStep. rewrite FS.in_union_iff, FS.in_bind_iff.
-  pose proof propagateTable_invariant as
-    [_ [_ [_ [_ [_ SOUND_IN]]]]]. split.
-  - intros [SEED | (y & EDGE & IN)].
-    + now eapply propagate_closure_on_seed.
-    + eapply propagate_closure_on_step with (y := y).
-      * exact EDGE.
-      * unfold tableGet in IN.
-        destruct (lookup y propagateTable) as [row | ] eqn:LOOK;
-          [ | contradiction IN].
-        pose proof propagateTable_invariant as [_ [KEYS _]].
-        exact (KEYS y row LOOK).
-      * now eapply SOUND_IN.
-  - intros CLOSURE. destruct CLOSURE as [SEED | y EDGE IN_Y CLOSURE].
-    + now left.
-    + right. exists y. split; [exact EDGE | ].
-      exact (propagateTable_complete_on y a IN_Y CLOSURE).
+  revert fuel1 x a LE IN; induction fuel2 as [ | fuel2 IH]; intros fuel1 x a LE IN.
+  - assert (fuel1 = O) as EQ by lia. subst fuel1. exact IN.
+  - pose proof (Nat.eq_dec fuel1 (S fuel2)) as [EQ | NE].
+    + subst fuel1. exact IN.
+    + eapply propagate_value_monotone_step.
+      eapply IH with (fuel1 := fuel1) (x := x) (a := a); [lia | exact IN].
 Qed.
 
-Theorem propagate_kleene_iff_closure (x : X) (a : A)
-  (deps_CLOSED : forall x : X, forall y : X, y ∈ deps x -> y ∈ nodes)
-  : a ∈ propagate_kleene x <-> x \in propagate_closure a.
+Theorem propagate_trace_value (x : X) (a : A) (tr : list X) (fuel : nat)
+  (TRACE : propagate_trace a x tr)
+  (LE : length tr <= fuel)
+  : a ∈ propagate_value fuel x.
 Proof.
-  unfold propagate_kleene, tableStep. rewrite FS.in_union_iff, FS.in_bind_iff.
-  pose proof propagateTable_invariant as [_ [_ [_ [_ [SOUND _]]]]]. split.
-  - intros [SEED | (y & EDGE & IN)].
-    + now eapply propagate_closure_seed.
-    + eapply propagate_closure_step with (y := y); [exact EDGE | ].
-      now eapply SOUND.
-  - intros CLOSURE. destruct CLOSURE as [SEED | y EDGE CLOSURE].
-    + now left.
-    + right. exists y. split; [exact EDGE | ].
-      exact (propagateTable_complete y a
-        (deps_CLOSED x y EDGE) CLOSURE deps_CLOSED).
+  revert fuel LE; induction TRACE as [x IN | x y tr EDGE TRACE IH]; intros fuel LE.
+  - now eapply propagate_value_seed.
+  - destruct fuel as [ | fuel]; simpl in LE; [lia | ].
+    eapply propagate_value_propagated; [exact EDGE | eapply IH; lia].
 Qed.
 
-Corollary propagate_kleene_equation
-  (deps_CLOSED : forall x : X, forall y : X, y ∈ deps x -> y ∈ nodes)
-  : propagate_equation propagate_kleene.
+Theorem propagate_closure_intro (x : X) (a : A)
+  (IN : x \in propagate_closure a)
+  : exists fuel, a ∈ propagate_value fuel x.
 Proof.
-  intros x a. unnw. rewrite propagate_kleene_iff_closure by exact deps_CLOSED. split.
-  - intros CLOSURE. destruct CLOSURE as [SEED_IN | y EDGE CLOSURE].
-    + now left.
-    + right. exists y. split; [exact EDGE | ].
-      rewrite propagate_kleene_iff_closure by exact deps_CLOSED. exact CLOSURE.
-  - intros [SEED_IN | (y & EDGE & IN)].
-    + now eapply propagate_closure_seed.
-    + rewrite propagate_kleene_iff_closure in IN by exact deps_CLOSED.
-      now eapply propagate_closure_step with (y := y).
+  induction IN as [x SEED_IN | x y EDGE CLOSURE IH].
+  - exists O. eapply propagate_value_seed. exact SEED_IN.
+  - destruct IH as [fuel VALUE_IN]. exists (S fuel). eapply propagate_value_propagated; eauto.
 Qed.
 
-Corollary propagate_kleene_least (value : X -> fset A) (x : X) (a : A)
-  (deps_CLOSED : forall x : X, forall y : X, y ∈ deps x -> y ∈ nodes)
-  (EQUATION : propagate_equation value)
-  (IN : a ∈ propagate_kleene x)
-  : a ∈ value x.
+Theorem propagate_closure_intro_bounded (fuel : nat) (nodes : fset X) (x : X) (a : A)
+  (fuel_ENOUGH : length nodes.(FSet.data) <= fuel)
+  (deps_CLOSED : forall x, forall y, y ∈ deps x -> y ∈ nodes)
+  (IN : x \in propagate_closure a)
+  : a ∈ propagate_value fuel x.
 Proof.
-  eapply propagate_closure_least; [exact EQUATION | ].
-  rewrite <- propagate_kleene_iff_closure by exact deps_CLOSED. exact IN.
+  rewrite propagate_closure_iff_trace in IN. destruct IN as [tr TRACE].
+  pose proof (propagate_trace_simple_bounded nodes x a tr deps_CLOSED TRACE) as (simple & TRACE' & LENGTH).
+  eapply propagate_trace_value with (tr := simple); [exact TRACE' | lia].
 Qed.
 
-End KLEENE.
+Theorem propagate_value_iff_closure_bounded (fuel : nat) (nodes : fset X) (x : X) (a : A)
+  (fuel_ENOUGH : length nodes.(FSet.data) <= fuel)
+  (deps_CLOSED : forall x, forall y, y ∈ deps x -> y ∈ nodes)
+  : a ∈ propagate_value fuel x <-> x \in propagate_closure a.
+Proof.
+  split.
+  - exact (propagate_value_elim fuel x a).
+  - intros IN. eapply propagate_closure_intro_bounded; eauto.
+Qed.
 
 End DIGRAPH.
 
-Section KLEENE_EXT.
-
-Context {X : Type} {POSET_X : isPoset X} {HsOrd_X : HsOrd X (POSET := POSET_X)}.
-Context {A : Type} {POSET_A : isPoset A} {HsOrd_A : HsOrd A (POSET := POSET_A)}.
-
-Lemma propagate_kleene_ext (seed : X -> fset A) (deps : X -> fset X) (deps' : X -> fset X) (nodes : fset X)
-  (EXT : forall x : X, deps x = deps' x)
-  : forall x : X, propagate_kleene seed deps nodes x = propagate_kleene seed deps' nodes x.
-Proof.
-  intros x. rewrite fset_eq_spec. intro a.
-  rewrite !propagate_kleene_iff_closure_on. split.
-  - intro CLOSURE. induction CLOSURE as
-      [x SEED | x y EDGE IN_Y CLOSURE IH].
-    + now eapply propagate_closure_on_seed.
-    + eapply propagate_closure_on_step with (y := y).
-      * rewrite <- (EXT x). exact EDGE.
-      * exact IN_Y.
-      * exact IH.
-  - intro CLOSURE. induction CLOSURE as
-      [x SEED | x y EDGE IN_Y CLOSURE IH].
-    + now eapply propagate_closure_on_seed.
-    + eapply propagate_closure_on_step with (y := y).
-      * rewrite (EXT x). exact EDGE.
-      * exact IN_Y.
-      * exact IH.
-Qed.
-
-Lemma propagate_kleene_ext_on (seed : X -> fset A) (deps : X -> fset X) (deps' : X -> fset X) (nodes : fset X)
-  (EXT : forall x : X, L.In x nodes.(FSet.data) -> deps x = deps' x)
-  : forall x : X, L.In x nodes.(FSet.data) -> (propagate_kleene seed deps nodes x = propagate_kleene seed deps' nodes x).
-Proof.
-  intros x IN_X. rewrite fset_eq_spec. intro a.
-  rewrite !propagate_kleene_iff_closure_on. split.
-  - intro CLOSURE. revert IN_X. induction CLOSURE as
-      [x SEED | x y EDGE IN_Y CLOSURE IH]; intros IN_X.
-    + now eapply propagate_closure_on_seed.
-    + eapply propagate_closure_on_step with (y := y).
-      * rewrite <- (EXT x IN_X). exact EDGE.
-      * exact IN_Y.
-      * exact (IH IN_Y).
-  - intro CLOSURE. revert IN_X. induction CLOSURE as
-      [x SEED | x y EDGE IN_Y CLOSURE IH]; intros IN_X.
-    + now eapply propagate_closure_on_seed.
-    + eapply propagate_closure_on_step with (y := y).
-      * rewrite (EXT x IN_X). exact EDGE.
-      * exact IN_Y.
-      * exact (IH IN_Y).
-Qed.
-
-Lemma propagate_kleene_seed_ext_on
-  (seed seed' : X -> fset A) (deps : X -> fset X) (nodes : fset X)
-  (CLOSED : forall x y : X,
-    L.In y (deps x).(FSet.data) -> L.In y nodes.(FSet.data))
-  (EXT : forall x : X,
-    L.In x nodes.(FSet.data) -> seed x = seed' x)
-  (x : X) (IN_X : L.In x nodes.(FSet.data))
-  : propagate_kleene seed deps nodes x =
-    propagate_kleene seed' deps nodes x.
-Proof.
-  rewrite fset_eq_spec. intro a.
-  rewrite !propagate_kleene_iff_closure by exact CLOSED.
-  split.
-  - intro CLOSURE. revert IN_X.
-    induction CLOSURE as [x SEED | x y EDGE CLOSURE IH]; intro IN_X.
-    + eapply propagate_closure_seed.
-      rewrite <- (EXT x IN_X). exact SEED.
-    + eapply propagate_closure_step with (y := y).
-      * exact EDGE.
-      * apply IH. eapply CLOSED. exact EDGE.
-  - intro CLOSURE. revert IN_X.
-    induction CLOSURE as [x SEED | x y EDGE CLOSURE IH]; intro IN_X.
-    + eapply propagate_closure_seed.
-      rewrite (EXT x IN_X). exact SEED.
-    + eapply propagate_closure_step with (y := y).
-      * exact EDGE.
-      * apply IH. eapply CLOSED. exact EDGE.
-Qed.
-
-End KLEENE_EXT.
-
 End DigraphFixedpoint.
-
-#[local] Notation "x '∈f' X" :=
-  (L.In x X.(FSet.data))
-  (at level 70, no associativity) : type_scope.
-
-Section FINITE_REACHABILITY.
-
-Context {A : Type} {A_isPoset : isPoset A}
-  {HsOrd_A : HsOrd A (POSET := A_isPoset)}.
-
-Variable V : fset A.
-Variable succ : A -> fset A.
-
-Definition succV (x : A) : fset A :=
-  inter (succ x) V.
-
-Lemma succV_sub (x : A) (z : A)
-  (IN : z ∈f succV x)
-  : z ∈f V.
-Proof.
-  unfold succV in IN.
-  exact (proj2 (proj1 (in_inter_iff (succ x) V z) IN)).
-Qed.
-
-#[local] Abbreviation RConfig := (list A * fset A)%type.
-
-Definition rok (c : RConfig) : Prop :=
-  (forall z : A, z ∈f snd c -> z ∈f V) /\
-  (forall z : A, L.In z (fst c) -> z ∈f V).
-
-Definition rstep (c : RConfig) : RConfig :=
-  match fst c with
-  | [] => c
-  | x :: xs =>
-    if FS.mem x (snd c) then
-      (xs, snd c)
-    else
-      (xs ++ (succV x).(FSet.data), FS.add x (snd c))
-  end.
-
-Definition rho (c : RConfig) : nat :=
-  (length V.(FSet.data) - length (snd c).(FSet.data)) *
-    (length V.(FSet.data) + 1) + length (fst c).
-
-Lemma rstep_rok (c : RConfig)
-  (H : rok c)
-  : rok (rstep c).
-Proof.
-  destruct c as [todo seen]. destruct H as [H_seen H_todo].
-  unfold rstep. cbn [fst snd] in *.
-  destruct todo as [ | x xs]; [split; assumption | ].
-  destruct (FS.mem x seen) as [ | ].
-  - split; cbn [fst snd]; [exact H_seen | ].
-    intros z z_in. eapply H_todo. now right.
-  - split; cbn [fst snd].
-    + intros z z_in. rewrite FS.in_add_iff in z_in.
-      destruct z_in as [EQ | z_in].
-      * subst z. eapply H_todo. now left.
-      * exact (H_seen z z_in).
-    + intros z z_in. rewrite L.in_app_iff in z_in.
-      destruct z_in as [z_in | z_in].
-      * eapply H_todo. now right.
-      * exact (succV_sub x z z_in).
-Qed.
-
-Lemma rstep_lt (c : RConfig) (x : A) (xs : list A)
-  (H : rok c)
-  (TODO : fst c = x :: xs)
-  : rho (rstep c) < rho c.
-Proof.
-  destruct c as [todo seen]. destruct H as [H_seen H_todo].
-  cbn [fst snd] in TODO. subst todo.
-  unfold rho, rstep. cbn [fst snd].
-  assert (SEEN_LE :
-    length seen.(FSet.data) <= length V.(FSet.data)).
-  { eapply fset_length_le. exact H_seen. }
-  destruct (FS.mem x seen) as [ | ] eqn: MEM.
-  - cbn [fst snd length]. lia.
-  - pose proof (proj1 (FS.mem_spec x seen false) MEM) as NOTIN.
-    clear MEM.
-    assert (X_IN : x ∈f V) by (eapply H_todo; now left).
-    assert (SEEN_LT :
-      length seen.(FSet.data) < length V.(FSet.data)).
-    { enough (WTS :
-        length (FS.add x seen).(FSet.data) <= length V.(FSet.data)).
-      { cbn [FS.add FSet.data] in WTS.
-        rewrite FS.length_insert in WTS by exact NOTIN. lia. }
-      eapply fset_length_le. intros z z_in.
-      rewrite FS.in_add_iff in z_in.
-      destruct z_in as [EQ | z_in];
-        [subst z; exact X_IN | exact (H_seen z z_in)].
-    }
-    assert (SUCC_LE :
-      length (succV x).(FSet.data) <= length V.(FSet.data)).
-    { eapply fset_length_le. exact (succV_sub x). }
-    cbn [fst snd]. rewrite L.length_app.
-    change (FS.add x seen).(FSet.data) with
-      (FS.insert x seen.(FSet.data)).
-    rewrite FS.length_insert by exact NOTIN.
-    cbn [length].
-    remember (length V.(FSet.data)) as v eqn: Hv.
-    remember (length seen.(FSet.data)) as s eqn: Hs.
-    remember (length (succV x).(FSet.data)) as k eqn: Hk.
-    destruct (v - s) as [ | d] eqn: HD; [lia | ].
-    replace (v - S s) with d by lia.
-    rewrite Nat.mul_succ_l. lia.
-Qed.
-
-Definition reachRun
-  : forall c : RConfig, rok c -> Acc Nat.lt (rho c) -> fset A.
-Proof.
-  refine (fix go (c : RConfig) (H : rok c)
-    (H_Acc : Acc Nat.lt (rho c)) {struct H_Acc} : fset A := _).
-  destruct (fst c) as [ | x xs] eqn: TODO.
-  - exact (snd c).
-  - exact (go (rstep c) (rstep_rok c H)
-      (Acc_inv H_Acc (rstep_lt c x xs H TODO))).
-Defined.
-
-Fixpoint reachRun_pirrel (c : RConfig)
-  (H1 : rok c) (H2 : rok c)
-  (H_Acc : Acc Nat.lt (rho c)) (H_Acc' : Acc Nat.lt (rho c)) {struct H_Acc}
-  : reachRun c H1 H_Acc = reachRun c H2 H_Acc'.
-Proof.
-  destruct c as [todo seen], todo as [ | x xs];
-    destruct H_Acc as [H_Acc_inv], H_Acc' as [H_Acc_inv']; cbn [reachRun].
-  - reflexivity.
-  - eapply reachRun_pirrel.
-Qed.
-
-Lemma reach_impl_rok (S0 : fset A)
-  : rok ((inter S0 V).(FSet.data), FS.empty).
-Proof.
-  split; cbn [fst snd].
-  - intros z z_in. destruct z_in.
-  - intros z z_in.
-    exact (proj2 (proj1 (in_inter_iff S0 V z) z_in)).
-Qed.
-
-Definition reach_impl (S0 : fset A) : fset A :=
-  reachRun ((inter S0 V).(FSet.data), FS.empty) (reach_impl_rok S0)
-    (accLt (rho ((inter S0 V).(FSet.data), FS.empty))).
-
-Fixpoint reachRun_sub (c : RConfig) (H : rok c)
-  (H_Acc : Acc Nat.lt (rho c)) {struct H_Acc}
-  : forall z : A, z ∈f reachRun c H H_Acc -> z ∈f V.
-Proof.
-  destruct c as [todo seen], todo as [ | x xs];
-    destruct H_Acc as [H_Acc_inv]; cbn [reachRun].
-  - exact (proj1 H).
-  - eapply reachRun_sub.
-Qed.
-
-Lemma reach_impl_sub (S0 : fset A) (z : A)
-  (IN : z ∈f reach_impl S0)
-  : z ∈f V.
-Proof.
-  exact (reachRun_sub _ _ _ z IN).
-Qed.
-
-Definition rstepStack (c : RConfig) : RConfig :=
-  match fst c with
-  | [] => c
-  | x :: xs =>
-    if FS.mem x (snd c) then
-      (xs, snd c)
-    else
-      ((succV x).(FSet.data) ++ xs, FS.add x (snd c))
-  end.
-
-Lemma rstepStack_rok (c : RConfig)
-  (H : rok c)
-  : rok (rstepStack c).
-Proof.
-  destruct c as [todo seen]. destruct H as [H_seen H_todo].
-  unfold rstepStack. cbn [fst snd] in *.
-  destruct todo as [ | x xs]; [split; assumption | ].
-  destruct (FS.mem x seen) as [ | ].
-  - split; cbn [fst snd]; [exact H_seen | ].
-    intros z z_in. eapply H_todo. now right.
-  - split; cbn [fst snd].
-    + intros z z_in. rewrite FS.in_add_iff in z_in.
-      destruct z_in as [EQ | z_in].
-      * subst z. eapply H_todo. now left.
-      * exact (H_seen z z_in).
-    + intros z z_in. rewrite L.in_app_iff in z_in.
-      destruct z_in as [z_in | z_in].
-      * exact (succV_sub x z z_in).
-      * eapply H_todo. now right.
-Qed.
-
-Lemma rstepStack_rho (c : RConfig)
-  : rho (rstepStack c) = rho (rstep c).
-Proof.
-  destruct c as [todo seen], todo as [ | x xs]; [reflexivity | ].
-  unfold rstepStack, rstep, rho. cbn [fst snd].
-  destruct (FS.mem x seen); [reflexivity | ].
-  cbn [fst snd]. rewrite !L.length_app. lia.
-Qed.
-
-Lemma rstepStack_lt (c : RConfig) (x : A) (xs : list A)
-  (H : rok c)
-  (TODO : fst c = x :: xs)
-  : rho (rstepStack c) < rho c.
-Proof.
-  rewrite rstepStack_rho. exact (rstep_lt c x xs H TODO).
-Qed.
-
-Definition reachRunStack
-  : forall c : RConfig, rok c -> Acc Nat.lt (rho c) -> fset A.
-Proof.
-  refine (fix go (c : RConfig) (H : rok c)
-    (H_Acc : Acc Nat.lt (rho c)) {struct H_Acc} : fset A := _).
-  destruct (fst c) as [ | x xs] eqn: TODO.
-  - exact (snd c).
-  - exact (go (rstepStack c) (rstepStack_rok c H)
-      (Acc_inv H_Acc (rstepStack_lt c x xs H TODO))).
-Defined.
-
-Fixpoint reachRunStack_sub (c : RConfig) (H : rok c)
-  (H_Acc : Acc Nat.lt (rho c)) {struct H_Acc}
-  : forall z : A, z ∈f reachRunStack c H H_Acc -> z ∈f V.
-Proof.
-  destruct c as [todo seen], todo as [ | x xs];
-    destruct H_Acc as [H_Acc_inv]; cbn [reachRunStack].
-  - exact (proj1 H).
-  - eapply reachRunStack_sub.
-Qed.
-
-Definition reach_impl_fast (S0 : fset A) : fset A :=
-  let c0 : RConfig := ((inter S0 V).(FSet.data), FS.empty) in
-  reachRunStack c0 (reach_impl_rok S0) (accLt (rho c0)).
-
-Lemma reach_impl_fast_sub (S0 : fset A) (z : A)
-  (IN : z ∈f reach_impl_fast S0)
-  : z ∈f V.
-Proof.
-  exact (reachRunStack_sub _ _ _ z IN).
-Qed.
-
-End FINITE_REACHABILITY.
-
-#[global] Arguments succV {A} {A_isPoset} {HsOrd_A} V succ x.
-#[global] Arguments rok {A} {A_isPoset} {HsOrd_A} V c.
-#[global] Arguments rstep {A} {A_isPoset} {HsOrd_A} V succ c.
-#[global] Arguments rho {A} {A_isPoset} {HsOrd_A} V c.
-#[global] Arguments reachRun {A} {A_isPoset} {HsOrd_A} V succ c H H_Acc.
-#[global] Arguments reach_impl {A} {A_isPoset} {HsOrd_A} V succ S0.
-#[global] Arguments rstepStack {A} {A_isPoset} {HsOrd_A} V succ c.
-#[global] Arguments rstepStack_rok
-  {A} {A_isPoset} {HsOrd_A} V succ c H.
-#[global] Arguments rstepStack_rho
-  {A} {A_isPoset} {HsOrd_A} V succ c.
-#[global] Arguments rstepStack_lt
-  {A} {A_isPoset} {HsOrd_A} V succ c x xs H TODO.
-#[global] Arguments reachRunStack
-  {A} {A_isPoset} {HsOrd_A} V succ c H H_Acc.
-#[global] Arguments reachRunStack_sub
-  {A} {A_isPoset} {HsOrd_A} V succ c H H_Acc z IN.
-#[global] Arguments reach_impl_fast
-  {A} {A_isPoset} {HsOrd_A} V succ S0.
-#[global] Arguments reach_impl_fast_sub
-  {A} {A_isPoset} {HsOrd_A} V succ S0 z IN.
